FastMultiplication.lean
@@ -3,6 +3,7 @@
 import FastMultiplication.ShorVerification.Implementation.Shor.Workspace
 import FastMultiplication.ShorVerification.Implementation.Shor.Correctness
 import FastMultiplication.ShorVerification.Implementation.PhaseProduct.Main
+import FastMultiplication.ShorVerification.Implementation.QFT.Main
 import FastMultiplication.ShorVerification.Implementation.GateCount.QFT_GateCount
 import FastMultiplication.ShorVerification.Implementation.GateCount.Shor_GateCount
 import FastMultiplication.ShorVerification.Framework.Submission
